Finished lambda case of the soundness proof. Morphism composition implemented as a right fold. Proof of a lemma about substitution of morphisms. Added bunch of lemmas relating different De Bruijn index manipulation functions.

forcing/Soundness.v
@@ -1,6 +1,6 @@
 Require Import Omega.
 Require Import Forcing.TemplateForcing.
-Require Import Template.Typing Template.Ast Template.WeakSubst Template.LiftSubst.
+Require Import Template.Typing Template.Ast Template.LiftSubst.
 From Template Require Export univ uGraph.
 
 Require Import String.
@@ -27,25 +27,103 @@ Definition ft_ctx Γ Σ σ  :=
 Definition ft_type_boxed c Σ σ  :=
   (snd (otranslate_boxed_type otranslate (Environ.of_global_context Σ) (mkFCtxt σ cat []) tt c)).
 
+Notation "'[' c ']ᵗ' " := (ft_term c) (at level 0).
+Notation "⟦ Γ ⟧" := (ft_ctx Γ)  (at level 40).
+Notation "'⟦' c '⟧ᵀ'" := (ft_type c) (at level 40).
+Notation "'⟦' c '⟧!'" := (ft_type_boxed c) (at level 40).
+
+Notation "Hom( a , b )" := (tApp cat.(cat_hom) [a;b]).
+
+Notation "fctx '.ₑ'" := (last_condition fctx) (at level 1, format "fctx .ₑ").
+Notation "dom( fctx , n )" := (get_domain_var fctx n) (at level 1).
+
+Definition tID q := tApp (tConst "Id_hom" []) [q].
+Notation "# q" := (tID q) (at level 51).
+Notation "g ∘ f <:: xs " := (tApp (tConst "Comp" []) (xs ++ [g;f])) (at level 49).
+Notation "fctx '.ₚ'" := (first_condition fctx) (at level 1, format "fctx .ₚ").
+Definition fctx_size := first_condition.
+Notation "^ i" := (tRel i) (at level 50, format "^ i").
+
+(* Forcing context extension *)
+Definition f_ctx_ext (σ σ' : list forcing_condition) := σ' ++ σ.
+Notation "σ ∙ σ' " := (f_ctx_ext σ σ') (at level 100).
+
 
 Definition leq_refl sigma t : leq_term sigma t t = true.
+Proof.
   induction t.
 Admitted.
 
-Definition cat_obj := tConst "Obj" [].
-Definition cat_hom := tConst "Hom" [].
-Definition id_hom := tConst "Id_hom" [].
-Definition sort_set := tSort [Universe.Expr.set].
+Definition eq_term_refl sigma t : eq_term sigma t t = true.
+Proof.
+Admitted.
+
+Lemma compare_string_refl s : compare_string s s = Eq.
+Proof.
+  unfold compare_string. rewrite Nat.compare_refl. reflexivity.
+Qed.
+
+Lemma univ_expr_eq_refl a : Universe.Expr.equal a a = true.
+Proof.
+  destruct a. simpl.
+  induction t;destruct b;simpl; try reflexivity;
+  try (unfold  Universe.Expr.equal,Level.equal;simpl;
+       try (rewrite compare_string_refl); (try rewrite Nat.compare_refl); reflexivity).
+Qed.
+
+Lemma leq_universe_refl uG s :
+  leq_universe uG s s = true.
+Proof.
+  unfold leq_universe.
+  assert (HH : Universe.equal s s = true).
+  { induction s.
+    + reflexivity.
+    + simpl. rewrite univ_expr_eq_refl. rewrite IHs. reflexivity. }
+  rewrite HH;reflexivity.
+Qed.
+
+Definition rlv_obj := Relevant.
+Definition rlv_hom := Relevant.
+Definition obj_univ := [Universe.Expr.set].
+Definition hom_univ := [Universe.Expr.set].
+Definition obj_sort := tSort obj_univ.
+Definition hom_sort := tSort hom_univ.
+Definition comp_type r_obj r_hom a b c :=
+  tProd a r_obj cat.(cat_obj)
+      (tProd b r_obj cat.(cat_obj)
+           (tProd c r_obj cat.(cat_obj)
+               (tProd nAnon r_hom Hom(^1,^0)
+                  (tProd nAnon r_hom Hom(^3,^2)
+                     Hom(^4,^2))))).
 
 (** We assume the following sorts for the objects and morphisms of the base category *)
-Axiom obj_sort : forall Σ Γ, Σ ;;; Γ |- cat_obj : sort_set.
-Axiom hom_sort : forall Σ Γ t1 t2,
-    Σ ;;; Γ |- t1 : cat_obj ->
-    Σ ;;; Γ |- t2 : cat_obj ->
-    Σ ;;; Γ |- tApp cat_hom [t1; t2] : sort_set.
+Axiom obj_sort_type : forall Σ Γ, Σ ;;; Γ |- cat.(cat_obj) : obj_sort.
+Axiom hom_sort_type : forall Σ Γ t1 t2,
+    Σ ;;; Γ |- t1 : cat.(cat_obj) ->
+    Σ ;;; Γ |- t2 : cat.(cat_obj) ->
+    Σ ;;; Γ |- tApp cat.(cat_hom) [t1; t2] : hom_sort.
 Axiom id_hom_type : forall Σ Γ t,
-    Σ ;;; Γ |- t : cat_obj ->
-    Σ ;;; Γ |- tApp id_hom [t] : tApp cat_hom [t; t].
+    Σ ;;; Γ |- t : cat.(cat_obj) ->
+    Σ ;;; Γ |- tApp cat.(cat_id) [t] : tApp cat.(cat_hom) [t; t].
+
+Quote Definition bazz := (forall a b c, b <= c -> a <= b -> a <= c).
+
+Axiom cat_comp_type : forall r_obj r_hom a b c Σ Γ,
+    Σ ;;; Γ |- cat.(cat_comp) : comp_type r_obj r_hom a b c.
+
+(* We define [weakening] as an axiom, because weakening in [Typing.v]
+   contains an assumption about well-formedness of the context and it
+   is not clear is it is needed (the proof if weakening is not
+   finished.) *)
+Axiom weakening : forall uG (Σ := ([], uG)) Γ Γ' (t : term) T,
+  wf_graph (snd Σ) ->
+  Σ ;;; Γ |- t : T ->
+  Σ ;;; Γ ,,, Γ' |- lift0 #|Γ'| t : lift0 #|Γ'| T.
+
+Axiom weakening_cumul : forall uG (Σ := ([], uG)) Γ Γ' (t u : term),
+    wf_graph (snd Σ) ->
+    Σ ;;; Γ |- t <= u ->
+    Σ ;;; Γ ,,, Γ' |- lift0 #|Γ'| t <= lift0 #|Γ'| u.
 
 Lemma wf_init_graph : wf_graph init_graph.
 Proof.
@@ -58,12 +136,14 @@ Proof.
       apply SetoidList.InA_cons_hd; auto.
       simpl. apply SetoidList.InA_cons_hd; eauto.
       (* NOTE: something is not right, either [wf_graph] or [init_graph] *)
+      (* In Coq the constraint is [lt], so it's better to fix [wf_graph] *)
 Admitted.
 
-Lemma typed_empty_global_env :
-  type_global_env init_graph [].
+Lemma typed_empty_global_env uG :
+  wf_graph uG ->
+  type_global_env uG [].
 Proof.
-  constructor. apply wf_init_graph.
+  constructor; auto.
 Qed.
 
 Ltac setctx na :=
@@ -74,7 +154,7 @@ Ltac setctx na :=
 
 Ltac setctx_2 na :=
   match goal with
-    |- ?Σ ;;; ?Γ ,, ?v2 ,, ?v1 |- _ : _ => set(na := [v1;v2])
+    |- ?Σ ;;; ?v1 :: ?v2 :: ?Γ |- _ : _ => set(na := [v1;v2])
   | |- type_local_env ?Σ ?Γ => match Γ with
                                | ?v1 :: ?v2 :: _ => set(na := [v1;v2])
                                end
@@ -91,115 +171,96 @@ Ltac solve_rel :=
     subst; apply type_Rel with (isdecl:=H')
   end.
 
-Reserved Notation "E ## Γ |= σ" (at level 40).
+Reserved Notation "E ## Γ => Γ' |= σ" (at level 40).
 
 (* TODO: think about the empty context case *)
-Inductive fctx_valid E : context -> list forcing_condition -> Type :=
-| fctx_valid_nil : E ## vass (nNamed "p") Relevant (tConst "Obj" nil) :: nil |= nil
-| fctx_valid_cons_var Γ σ T : E ## Γ |= σ ->
-                            E ## (Γ ,, vass (nNamed "t") Relevant T) |= (σ ,, fcVar)
-| fctx_valid_cons_lift Γ σ : E ## Γ |= σ ->
-                        E ## (Γ ,,, get_ctx_lift cat E (last_condition σ)) |= (σ ,, fcLift)
-where "E ## Γ |= σ" := (fctx_valid E Γ σ).
+Inductive fctx_valid E : context -> context -> list forcing_condition -> Type :=
+| fctx_valid_nil : E ## [] => [vass (nNamed "p") rlv_obj (tConst "Obj" nil)] |= nil
+| fctx_valid_cons_var Γ Γ' σ T n n' r r':
+    E ## Γ => Γ' |= σ ->
+    let v := vass n r T in
+    let T' := ⟦T⟧! (to_global_context E) σ in
+    let v' := vass n' r' T' in
+        E ## (Γ ,, v) => (Γ' ,, v') |= (σ ,, fcVar)
+| fctx_valid_cons_lift Γ Γ' σ :
+    E ## Γ => Γ' |= σ ->
+    E ## Γ => (Γ' ,,, get_ctx_lift cat E (last_condition σ)) |= (σ ,, fcLift)
+where "E ## Γ => Γ' |= σ" := (fctx_valid E Γ Γ' σ).
 
 
-Lemma last_condition_sound σ Γ (Σ := ([], init_graph)) :
-  type_local_env Σ Γ ->
-  (of_global_context Σ) ## Γ |= σ ->
-  Σ ;;; Γ |- tRel (last_condition σ) : cat_obj.
+Lemma last_condition_sound σ Γ Γ' uG (Σ := ([], uG)) :
+  wf_graph uG ->
+  (of_global_context Σ) ## Γ => Γ' |= σ ->
+  Σ ;;; Γ' |- tRel (last_condition σ) : cat.(cat_obj).
 Proof.
-  intros TyCtx FcValid.
+  intros wfG FcValid.
   induction FcValid.
-  - simpl. solve_rel.
+  - cbv. solve_rel.
   - simpl.
-    pose [vass (nNamed "t") Relevant T] as Γ'.
-    change (Σ;;; Γ ,,, Γ' |- lift0 #|Γ'| (tRel (last_condition σ)) : lift0 #|Γ'| (cat_obj)).
-    assert (TyCtxΓ : type_local_env Σ Γ).
-    { inversion TyCtx;subst;auto. }
+    change (Σ;;; Γ' ,,, [v'] |- lift0 1 (tRel (last_condition σ)) : lift0 1 cat.(cat_obj)).
     apply weakening.
-    + apply typed_empty_global_env.
-    + simpl.
-      (* NOTE: here we do inversion again, because of some issues with [typing] being in [Type] *)
-      inversion TyCtx;subst;auto.
-    + apply IHFcValid; eauto.
+    + exact wfG.
+    + exact IHFcValid.
   - solve_rel.
 Qed.
 
-Lemma lift_sound (Σ := (nil,init_graph)) Γ σ v :
-  type_local_env Σ Γ ->
-  (of_global_context Σ) ## Γ |= σ ->
-  Σ;;; Γ,, vass v Relevant cat_obj |- tApp cat_hom [tRel (S (last_condition σ)); tRel 0] : sort_set.
+Lemma lift_sound uG (Σ := (nil,uG)) Γ Γ' σ v :
+  wf_graph uG ->
+  (of_global_context Σ) ## Γ => Γ' |= σ ->
+  Σ;;; Γ',, vass v rlv_obj cat.(cat_obj) |- Hom(^(1+σ.ₑ),^0) : obj_sort.
 Proof.
-  intros TyCtx FcValid.
-  eapply hom_sort.
-  - pose ([vass v Relevant cat_obj]) as Γ'.
+  intros wfG FcValid.
+  eapply hom_sort_type.
+  - pose ([vass v rlv_obj cat.(cat_obj)]) as Γ''.
     change
-      (Σ;;; Γ ,,, Γ' |- lift0 #|Γ'| (tRel (last_condition σ)) : lift0 #|Γ'| cat_obj).
-    apply weakening with (Γ' := Γ').
-    * apply typed_empty_global_env.
-    * simpl. constructor. apply TyCtx. econstructor. simpl. apply obj_sort.
-    * apply last_condition_sound;eauto.
+      (Σ;;; Γ' ,,, Γ'' |- lift0 #|Γ''| (tRel (last_condition σ)) : lift0 #|Γ''| cat.(cat_obj)).
+    apply weakening with (Γ' := Γ'').
+    * exact wfG.
+    * apply last_condition_sound with (Γ := Γ);eauto.
   - solve_rel.
 Qed.
 
-Lemma lam_q_f_sound (Σ := (nil,init_graph)) Γ σ t T :
+Lemma lam_q_f_sound uG (Σ := (nil,uG)) Γ Γ' σ t T :
   let E := (of_global_context Σ) in
   let fctx := (mkFCtxt σ cat []) in
   let ext := get_ctx_lift cat E (last_condition σ) in
-  type_local_env Σ Γ ->
-  (of_global_context Σ) ## Γ |= σ ->
-  Σ ;;; Γ ,,, ext |- t : T ->
-  Σ ;;; Γ |- snd (λ_q_f E fctx) t : snd (Π_q_f E fctx) T.
+  wf_graph uG ->
+  (of_global_context Σ) ## Γ => Γ' |= σ ->
+  Σ ;;; Γ' ,,, ext |- t : T ->
+  Σ ;;; Γ' |- snd (λ_q_f E fctx) t : snd (Π_q_f E fctx) T.
 Proof.
-  simpl. intros TyCtx FcValid Ty.
+  simpl. intros wfG FcValid Ty.
   econstructor.
-  + eapply obj_sort.
+  + eapply obj_sort_type.
   + econstructor.
-    * apply lift_sound;eauto.
+    * eapply lift_sound;eauto.
     * eauto.
 Qed.
 
-Lemma Π_q_f_lift_sound (Σ := (nil,init_graph)) Γ σ T l :
+Lemma Π_q_f_lift_sound uG (Σ := (nil,uG)) Γ σ T s :
   let σ_ext := σ ,, fcLift in
   let fctx_ext := (mkFCtxt σ_ext cat []) in
   let E := (of_global_context Σ) in
   let ext1 := get_ctx_lift cat E (last_condition σ) in
   let ext2 := get_ctx_lift cat E (last_condition σ_ext) in
-  Σ ;;; Γ ,,, ext1 ,,, ext2  |- T : tSort l ->
+  wf_graph uG ->
+  Σ ;;; Γ ,,, ext1 ,,, ext2  |- T : tSort s ->
   Σ ;;; Γ ,,, ext1 |- snd (Π_q_f E fctx_ext) T :
-  tSort (Universe.sup [Universe.Expr.set]  (Universe.sup [Universe.Expr.set] l)).
+  tSort (Universe.sup obj_univ (Universe.sup hom_univ s)).
 Proof.
   simpl.
-  intros H.
+  intros wfG H.
   apply type_Prod.
-  ** apply obj_sort.
+  ** apply obj_sort_type.
   ** apply type_Prod.
-     *** apply hom_sort; solve_rel.
+     *** apply hom_sort_type; solve_rel.
      *** eauto.
 Qed.
 
-Notation "'[' c ']ᵗ' " := (ft_term c) (at level 0).
-Notation "⟦ Γ ⟧" := (ft_ctx Γ)  (at level 40).
-Notation "'⟦' c '⟧ᵀ'" := (ft_type c) (at level 40).
-Notation "'⟦' c '⟧!'" := (ft_type_boxed c) (at level 40).
+(* Lemma forcing_context_soundness Σ Γ σ : *)
+(*   type_local_env Σ Γ -> type_local_env Σ (⟦Γ⟧ Σ σ). *)
+(* Admitted. *)
 
-Lemma context_traslation_valid E Γ σ :
-  let Σ := to_global_context E in
-  type_local_env Σ Γ ->
-  E ## (⟦Γ⟧ Σ σ) |= σ.
-Proof.
-  intros ? TyCtx.
-  Admitted.
-
-Lemma forcing_context_soundness Σ Γ σ :
-  type_local_env Σ Γ -> type_local_env Σ (⟦Γ⟧ Σ σ).
-Admitted.
-
-
-Tactic Notation "solve_last_cond" :=
-  apply last_condition_sound;
-  [apply forcing_context_soundness;assumption |
-   apply context_traslation_valid;assumption].
 
 Ltac type_spine_step :=
   match goal with
@@ -208,36 +269,36 @@ Ltac type_spine_step :=
       [eapply cumul_refl;apply leq_refl | | ]
   end.
 
-Lemma sort_translation_prefix_sound (Σ := (nil,init_graph)) σ Γ T l:
+Lemma sort_translation_prefix_sound uG (Σ := (nil,uG)) σ Γ Γ' T s:
   let E := (of_global_context Σ) in
   let fctx := (mkFCtxt σ cat []) in
-  let srt := tSort (Universe.sup [Universe.Expr.set]  (Universe.sup [Universe.Expr.set] l)) in
+  let srt := tSort (Universe.sup obj_univ  (Universe.sup hom_univ s)) in
   let ext1 := get_ctx_lift cat E (last_condition σ) in
   let ext2 := get_ctx_lift cat E (last_condition (σ ,, fcLift)) in
-  type_local_env Σ Γ ->
-  (of_global_context Σ) ## Γ |= σ ->
-  Σ ;;; Γ ,,, ext1 ,,, ext2  |- T : tSort l ->
-  Σ ;;; Γ |- snd (sort_translation_prefix E fctx tt) T
+  wf_graph uG ->
+  (of_global_context Σ) ## Γ => Γ' |= σ ->
+  Σ ;;; Γ' ,,, ext1 ,,, ext2  |- T : tSort s ->
+  Σ ;;; Γ' |- snd (sort_translation_prefix E fctx tt) T
                       : snd (Π_q_f E fctx) srt.
 Proof.
-  intros ? ? ? ? ? TyCtx FcValid TyT.
+  intros ? ? ? ? ? wfG FcValid TyT.
   simpl.
-  apply lam_q_f_sound;simpl;eauto.
-  unfold sort_set.
-  eapply Π_q_f_lift_sound. apply TyT.
+  eapply lam_q_f_sound;simpl;eauto.
+  unfold obj_sort.
+  eapply Π_q_f_lift_sound;auto.
 Qed.
 
-Lemma type_translation_sound (Σ := ([],init_graph)) Γ σ T :
-  type_local_env Σ Γ ->
-  (of_global_context Σ) ## Γ |= σ ->
-  Σ;;; Γ |- [T ]ᵗ Σ σ : (⟦ tSort [Universe.Expr.set] ⟧ᵀ) Σ σ ->
-  Σ ;;; Γ |- ⟦T⟧ᵀ Σ σ : tSort [Universe.Expr.set].
+Lemma type_translation_sound uG (Σ := ([],uG)) Γ Γ' σ T s:
+  wf_graph uG ->
+  (of_global_context Σ) ## Γ => Γ' |= σ ->
+  Σ;;; Γ' |- [T ]ᵗ Σ σ : (⟦ tSort s ⟧ᵀ) Σ σ ->
+  Σ ;;; Γ' |- ⟦T⟧ᵀ Σ σ : tSort s.
 Proof.
-  intros TyCtx FcValid TyT.
+  intros wfG FcValid TyT.
   unfold ft_type,otranslate_type. simpl. unfold mkOptApp.
   remember (tRel (last_condition σ)) as last_fcond.
   remember (tApp (tConst "Id_hom" []) [last_fcond]) as id_hom_lfc.
-  change (Σ;;; Γ |- tApp ([T]ᵗ Σ σ) [last_fcond; id_hom_lfc] : tSort [Universe.Expr.set]).
+  (* change (Σ;;; Γ' |- tApp ([T]ᵗ Σ σ) [last_fcond; id_hom_lfc] : tSort [Universe.Expr.set]). *)
   eapply type_App.
   - eapply TyT.
   - unfold ft_type. simpl. unfold mkOptApp. econstructor.
@@ -247,165 +308,1276 @@ Proof.
       eapply cumul_red_r. Focus 2.
       eapply red_beta. simpl.
       eapply cumul_refl. apply leq_refl.
-    * subst. apply last_condition_sound;eauto.
+    * subst. eapply last_condition_sound;eauto.
     * econstructor. Focus 2.
-      subst. apply id_hom_type. apply last_condition_sound;eauto.
+      subst. apply id_hom_type. eapply last_condition_sound; eassumption.
       econstructor. subst. eapply leq_refl.
       econstructor.
 Qed.
 
-Lemma ctx_with_lift_sound (Σ := ([],init_graph)) Γ σ:
+Lemma ctx_with_lift_sound (Σ := ([],init_graph)) Γ Γ' σ:
   let ext := get_ctx_lift cat (of_global_context Σ) (last_condition σ) in
-  type_local_env Σ Γ ->
-  (of_global_context Σ) ## Γ |= σ ->
-  type_local_env Σ (Γ ,,, ext).
+  type_local_env Σ Γ' ->
+  (of_global_context Σ) ## Γ => Γ' |= σ ->
+  type_local_env Σ (Γ' ,,, ext).
 Proof.
   simpl. intros TyCtx FcValid.
   constructor;eauto.
   constructor;eauto.
-  econstructor; apply obj_sort.
-  econstructor; apply lift_sound;eauto.
+  econstructor; apply obj_sort_type.
+  econstructor; eapply lift_sound;eauto.
+  apply wf_init_graph.
 Qed.
 
-Lemma boxed_type_translation_sound (Σ := ([],init_graph)) Γ σ A :
+
+Ltac change_type T :=
+  match goal with
+    [ |- ?Σ ;;; ?Γ |- ?t : ?T0 ] => change (Σ ;;; Γ |- t : T)
+  end.
+
+Notation "u1 ⊔ u2" := (Universe.sup u1 u2) (at level 40).
+
+Lemma boxed_type_translation_sound uG (Σ := ([],uG)) Γ Γ' σ A s :
   let ext := get_ctx_lift cat (of_global_context Σ) (last_condition σ) in
-  type_local_env Σ Γ ->
-  (of_global_context Σ) ## Γ |= σ ->
-  Σ ;;; Γ ,,, ext |- [A]ᵗ Σ (σ ,, fcLift) : (⟦ tSort [Universe.Expr.set] ⟧ᵀ) Σ (σ ,, fcLift) ->
-  Σ ;;; Γ |- ⟦A⟧! Σ σ :  tSort (Universe.sup [Universe.Expr.set] [Universe.Expr.set]).
+  wf_graph uG ->
+  (of_global_context Σ) ## Γ => Γ' |= σ ->
+  Σ ;;; Γ' ,,, ext |- [A]ᵗ Σ (σ ,, fcLift) : (⟦ tSort s ⟧ᵀ) Σ (σ ,, fcLift) ->
+  Σ ;;; Γ' |- ⟦A⟧! Σ σ :  tSort (obj_univ ⊔ (hom_univ ⊔ s)).
 Proof.
   simpl.
-  intros TyCtx FcValid H.
+  intros wfG FcValid H.
+  (* change_type (tSort (Universe.sup [Universe.Expr.set] [Universe.Expr.set])). *)
   unfold ft_type_boxed,otranslate_boxed_type. simpl.
   destruct (otranslate_type otranslate (of_global_context Σ)
             (extend_forcing_ctx {| f_context := σ; f_category := cat; f_translator := [] |} fcLift)
             tt A) eqn: HA.
   simpl. eapply type_Prod.
-  - apply obj_sort.
+  - apply obj_sort_type.
   - replace ([Universe.Expr.set]) with
         (Universe.sup [Universe.Expr.set] [Universe.Expr.set]) by reflexivity.
     eapply type_Prod.
-    pose ([vass pos_name Relevant (tConst "Obj" [])]) as Γ'.
-    eapply hom_sort.
-    + change (Σ;;; Γ ,,, Γ' |- lift0 #|Γ'| (tRel (last_condition σ)) : lift0 #|Γ'| (cat_obj)).
+    pose ([vass pos_name rlv_obj cat.(cat_obj)]) as Γ''.
+    eapply hom_sort_type.
+    + change (Σ;;; Γ' ,,, Γ'' |- lift0 #|Γ''| (tRel (last_condition σ)) : lift0 #|Γ''| (cat.(cat_obj))).
       subst Σ. eapply weakening.
-      * apply typed_empty_global_env.
-      * simpl. constructor;eauto.
-        econstructor. apply obj_sort.
-      * apply last_condition_sound;eauto.
+      * exact wfG.
+      * eapply last_condition_sound;eauto.
     + solve_rel.
-    + unfold mkOptApp. apply type_translation_sound.
-      * apply  ctx_with_lift_sound;eauto.
-      * constructor. assumption.
+    + unfold mkOptApp. eapply type_translation_sound.
+      * exact wfG.
+      * constructor. eassumption.
       * apply H.
 Qed.
 
-(* Lemma ctx_translation_extension (Σ := ([],init_graph)) σ Γ : *)
-(*   let E := of_global_context Σ in *)
-(*   ⟦ Γ ⟧ Σ (σ,, fcLift) = Γ ,,, (get_ctx_lift cat E (last_condition σ)). *)
-(* Proof. *)
-(*   simpl. destruct Γ. *)
-(*   - unfold ft_ctx,otranslate_context_no_sigma. simpl. cbv. *)
+Open Scope type_scope.
 
-Lemma forcing_typing_soundness (Σ := ([],init_graph)) Γ t T σ  :
+Definition lt_universe uG u1 u2 : bool := check_lt uG u1 u2.
+
+Axiom type_Sort_s :
+  forall Γ Σ s s', lt_universe (snd Σ) s s' = true -> Σ;;; Γ |- tSort s : tSort s'.
+
+(* This is not quite true, because one can take uG to be [init_graph] *)
+Axiom higher_universe_exists :
+  forall uG s, wf_graph uG -> {s' | (lt_universe uG s s' = true)}.
+
+Lemma univ_cumul uG (Σ := ([],uG)) Γ s s' s'' T:
+  leq_universe uG s s' = true ->
+  Σ;;; Γ |- T : tSort s ->
+  Σ;;; Γ |- tSort s' : tSort s'' ->
+  Σ;;; Γ |- T : tSort s'.
+Proof.
+  intros Hleq Hty Hsort.
+  eapply type_Conv;simpl.
+  + apply Hty.
+  + eauto.
+  + constructor. simpl. apply Hleq.
+Qed.
+
+Lemma translation_of_sort_sound uG (Σ := ([],uG)) Γ Γ' σ  s s' s'':
+  wf_graph uG ->
+  (of_global_context Σ) ## Γ => Γ' |= σ ->
+  lt_universe uG s s' = true ->
+  leq_universe uG (obj_univ ⊔ (hom_univ ⊔ s')) s'' = true ->
+   Σ;;; Γ' |- [tSort s ]ᵗ Σ σ : (⟦ tSort s''⟧ᵀ) Σ σ.
+Proof.
+  intros wfG FcValid Huniv Huniv'.
+  destruct (higher_universe_exists uG s'' wfG) as [s''' ?].
+  (* Simplifying the applications in the type first*)
+  unfold ft_term,otranslate,lambda_prefix,extend. cbn.
+  eapply type_Conv;simpl.
+  * eapply lam_q_f_sound;simpl.
+    ** assumption.
+    ** eassumption.
+    ** eapply Π_q_f_lift_sound.
+       *** exact wfG.
+       *** apply type_Sort_s;eauto.
+  * unfold ft_type. simpl in *. unfold mkOptApp.
+    eapply type_App.
+    ** eapply lam_q_f_sound;simpl.
+       *** assumption.
+       *** eassumption.
+       *** apply Π_q_f_lift_sound.
+           exact wfG.
+           apply type_Sort_s with (s':=s''');eauto.
+    ** simpl. (* typing_spine *)
+           type_spine_step. eapply last_condition_sound;eauto.
+           type_spine_step. apply id_hom_type. eapply last_condition_sound;eauto.
+           apply type_spine_nil.
+  * simpl. unfold ft_type. simpl. unfold mkOptApp.
+    (* Abstract this reduction to a tactic *)
+    eapply cumul_red_r. Focus 2.
+    eapply red_beta. simpl.
+    eapply cumul_red_r. Focus 2.
+    eapply red_beta. simpl.
+    eapply cumul_refl.
+    simpl. rewrite Huniv'.
+    (* rewrite leq_universe_refl. *)
+    rewrite Nat.eqb_refl. reflexivity.
+Qed.
+
+Lemma unit_unique : forall t : unit, t = tt.
+Proof. intros t;destruct t;reflexivity. Qed.
+
+Lemma lt_universe_leq uG s1 s2 : lt_universe uG s1 s2 = true -> leq_universe uG s1 s2 = true.
+Proof.
+Admitted.
+
+Lemma typed_term_sort uG (Σ := ([],uG)) Γ t T:
   type_local_env Σ Γ ->
+  wf_graph uG ->
+  Σ ;;; Γ |- t : T ->
+  {s : universe &  Σ ;;; Γ |- T : tSort s}.
+Proof.
+  intros TyCtx wfG Ty.
+  induction Ty.
+  - (* Use [TyCtx] and something like [rewrite Checker.nth_error_Some_safe_nth.] *)
+    admit.
+  - admit.
+  - auto.
+Admitted.
+
+Lemma prod_translation_sound uG (Σ := ([],uG)) (Σ' := Σ) Γ Γ' σ A B n s1 s2 r :
+  let ext := get_ctx_lift cat (of_global_context Σ) (last_condition σ) in
+  let σ' := (σ ,, fcLift) in
+  let ext1 := get_ctx_lift cat (of_global_context Σ) (last_condition σ') in
+  let v := vass n r (⟦A⟧! Σ (σ ,, fcLift)) in
+  wf_graph uG ->
+  (of_global_context Σ) ## Γ => Γ' |= σ ->
+  Σ';;; Γ' ,,, ext ,,, ext1 |- [A]ᵗ Σ (σ' ,, fcLift) : (⟦ tSort s1 ⟧ᵀ) Σ (σ' ,, fcLift) ->
+  Σ';;; Γ' ,,, ext ,, v |- [B]ᵗ Σ (σ' ,, fcVar) : (⟦ tSort s2 ⟧ᵀ) Σ (σ' ,, fcVar) ->
+  Σ;;; Γ' |- [tProd n r A B ]ᵗ Σ σ : (⟦ tSort (s1 ⊔ s2) ⟧ᵀ) Σ σ.
+Proof.
+  intros ? ? ? ? wfG FcValid TyA TyB.
+      unfold ft_type, ft_term.
+    (* pose (get_ctx_lift cat (of_global_context Σ) (last_condition σ)) as ext. *)
+    (* We first prove that boxed translation of a domain is sound, because we will use this fact
+       two times later. *)
+    assert (A_boxed: Σ ;;; Γ' ,,, ext |- ⟦A⟧! Σ σ' : tSort (obj_univ ⊔ (hom_univ ⊔ s1))).
+    { eapply boxed_type_translation_sound.
+      * exact wfG.
+      * repeat constructor;eauto.
+      * apply TyA;eauto. }
+    destruct (higher_universe_exists uG (s1 ⊔ s2) wfG) as [s' ?].
+    destruct (higher_universe_exists uG (obj_univ ⊔ (hom_univ ⊔ s')) wfG) as [s'' Hs''].
+    eapply type_Conv.
+    * simpl. eapply lam_q_f_sound;simpl.
+      ** assumption.
+      ** eassumption.
+      ** apply type_Prod.
+         *** eapply A_boxed.
+         *** unfold mkOptApp. setctx Γ''.
+             assert (BT: Σ ;;; Γ'' |- ⟦B⟧ᵀ Σ (σ ,, fcLift ,, fcVar) : tSort s2).
+             { eapply type_translation_sound with (Γ := Γ,, vass n r A).
+               + exact wfG.
+               + subst Γ''. unfold snoc.
+                 eapply fctx_valid_cons_var with (σ:=σ ,, fcLift).
+                 constructor;auto.
+               + apply TyB;eauto.
+             }
+             (* NOTE: rewriting with [unit_unique] in the goal doesn't work, so
+                we rewrite in the assumption instead. *)
+             unfold ft_type in BT.
+             erewrite <- unit_unique in BT.
+             apply BT.
+    * apply lt_universe_leq in Hs''.
+      eapply type_translation_sound;eauto.
+      eapply translation_of_sort_sound;eauto.
+    * eapply cumul_red_r. Focus 2. simpl.
+      eapply red_beta. simpl.
+      eapply cumul_red_r. Focus 2.
+      eapply red_beta. simpl.
+      eapply cumul_refl.
+      simpl. rewrite Nat.eqb_refl. simpl.
+        (* NOTE: works for sure if [s1] or [s2] are [Set] *)
+        (* TODO : this is the only thing to fix, the rest is fine *)
+        (* reflexivity. *)
+        admit.
+Admitted.
+
+(* A version of the [prod_translation_sound] which assumes that *type* (ans not term)
+   translations are sound *)
+(* NOTE: the proof of the theorem [prod_translation_sound] should be an application of this theorem
+   with additional work to construct the premises *)
+Lemma prod_translation_sound_alt uG (Σ := ([],uG)) (Σ' := Σ) Γ Γ' σ A B n s1 s2 r :
+  let ext := get_ctx_lift cat (of_global_context Σ) (last_condition σ) in
+  let σ' := (σ ,, fcLift) in
+  let ext1 := get_ctx_lift cat (of_global_context Σ) (last_condition σ') in
+  let v := vass n r (⟦A⟧! Σ (σ ,, fcLift)) in
+  wf_graph uG ->
+  (of_global_context Σ) ## Γ => Γ' |= σ ->
+  Σ';;; Γ' ,,, ext |- ⟦A⟧! Σ (σ ,, fcLift) : tSort s1 ->
+  Σ';;; Γ' ,,, ext ,, v |- ⟦B⟧ᵀ Σ (σ ,, fcLift ,, fcVar) : tSort s2 ->
+  Σ;;; Γ' |- [tProd n r A B ]ᵗ Σ σ : (⟦ tSort (s1 ⊔ s2) ⟧ᵀ) Σ σ.
+Proof.
+  intros ? ? ? ? wfG FcValid TyA TyB.
+  unfold ft_type, ft_term.
+  destruct (higher_universe_exists uG (s1 ⊔ s2) wfG) as [s' ?].
+  destruct (higher_universe_exists uG (obj_univ ⊔ (hom_univ ⊔ s')) wfG) as [s'' Hs''].
+  eapply type_Conv.
+  * simpl. eapply lam_q_f_sound;simpl.
+    ** assumption.
+    ** eassumption.
+    ** apply type_Prod.
+       *** eapply TyA.
+       *** unfold mkOptApp. setctx Γ''.
+           unfold ft_type in TyB.
+           erewrite <- unit_unique in TyB.
+           eapply TyB.
+  * apply lt_universe_leq in Hs''.
+    eapply type_translation_sound;eauto.
+    eapply translation_of_sort_sound;eauto.
+  * unfold mkOptApp.
+    eapply cumul_red_r. Focus 2.
+      eapply red_beta. simpl.
+      eapply cumul_red_r. Focus 2.
+      eapply red_beta. simpl.
+      eapply cumul_refl.
+      simpl. rewrite Nat.eqb_refl. simpl.
+      (* NOTE: works for sure if [s1] or [s2] are [Set] *)
+      (* TODO : this is the only thing to fix, the rest is fine *)
+      (* reflexivity. *)
+      admit.
+Admitted.
+
+Definition cat_id_conv_r :=
+  forall Σ Γ a b f,
+    Σ ;;; Γ |- f ∘ (# a) <:: [a;a;b] : Hom(a,b) ->
+    (Σ ;;; Γ |- (f ∘ (# a) <:: [a;a;b]) = f).
+
+Definition cat_id_conv_l :=
+  forall Σ Γ a b f,
+    Σ ;;; Γ |- (# b) ∘ f <:: [a;b;b] : Hom(a,b) ->
+    (Σ ;;; Γ |- ((# b) ∘ f <:: [a;b;b]) = f).
+
+
+Lemma bin_app_typed Σ Γ u t1 t2 r1 r2 A B C nam1 nam2 :
+  Σ ;;; Γ |- t1 : A ->
+  Σ ;;; Γ |- t2 : B{0:=t1} ->
+  Σ ;;; Γ |- u : tProd nam1 r1 A (tProd nam2 r2 B C) ->
+  Σ ;;; Γ |- tApp u [t1;t2] : C {1:=t1} {0:=t2}.
+Proof.
+  intros HA HB Hu.
+  econstructor.
+  + eapply Hu.
+  + eapply type_spine_const with (na :=nNamed "b") (relevance:=r1) (A:=A).
+    * eapply cumul_refl. simpl in *. rewrite eq_term_refl. eapply leq_refl.
+    * assumption.
+    * eapply type_spine_const with (na :=nNamed "b") (relevance:=r2) (A:=B {0:= t1}).
+      ** eapply cumul_refl. simpl in *. rewrite eq_term_refl. eapply leq_refl.
+      ** assumption.
+      ** econstructor.
+Qed.
+
+Lemma composition_typed Σ Γ a b c g f :
+  Σ ;;; Γ |- a : cat.(cat_obj) ->
+  Σ ;;; Γ |- b : cat.(cat_obj) ->
+  Σ ;;; Γ |- c : cat.(cat_obj) ->
+  Σ ;;; Γ |- f : Hom(a,b) ->
+  Σ ;;; Γ |- g : Hom(b,c) ->
+  Σ ;;; Γ |- g ∘ f <:: [a;b;c] : Hom(a,c).
+Proof.
+  econstructor.
+    + eapply (cat_comp_type rlv_obj rlv_hom (nNamed "a") (nNamed "b") (nNamed "c")).
+    + eapply type_spine_const with (na :=nNamed "a") (A:=cat.(cat_obj)) (relevance:=rlv_obj).
+      - eapply cumul_refl. simpl in *. eapply leq_refl.
+      - assumption.
+      - simpl. eapply type_spine_const with (na :=nNamed "b") (A:=cat.(cat_obj))(relevance:=rlv_obj).
+        * eapply cumul_refl. simpl in *. eapply leq_refl.
+        * assumption.
+        * simpl. eapply type_spine_const with (na :=nNamed "c") (A:=cat.(cat_obj))
+                                              (relevance:=rlv_obj).
+           ** eapply cumul_refl. simpl in *. eapply leq_refl.
+           ** assumption.
+           ** simpl. pose (((lift0 1) b){0:=c}) as x. rewrite lift0_p.
+               eapply type_spine_const with (A:=Hom(x,c)).
+               *** eapply cumul_refl. subst x. simpl in *.
+                   repeat rewrite eq_term_refl. simpl. eapply leq_refl.
+               *** subst x. econstructor.
+                   **** eassumption.
+                   **** eapply hom_sort_type. cbn.
+                    Admitted.
+
+Lemma composition_id_typed Σ Γ r_obj r_hom :
+  let f := vass hom_name r_hom (tApp (tConst "Hom" []) [^1; ^0]) in
+  let q := vass pos_name r_obj (tConst "Obj" []) in
+  let p := vass pos_name r_obj (tConst "Obj" []) in
+  Σ;;; Γ ,,, [f;q;p] |- (# ^1) ∘ (^0) <:: [^2; ^1; ^1] : Hom( ^2, ^1).
+Proof.
+  intros ? ?.
+  econstructor.
+    + eapply (cat_comp_type r_obj r_hom (nNamed "a") (nNamed "b") (nNamed "c")).
+    + eapply type_spine_const with (na :=nNamed "a") (A:=cat.(cat_obj)) (relevance:=r_obj).
+      - eapply cumul_refl. simpl in *. eapply leq_refl.
+      - solve_rel.
+      - eapply type_spine_const with (na :=nNamed "b") (A:=cat.(cat_obj)) (relevance:=r_obj).
+        * eapply cumul_refl. simpl in *. eapply leq_refl.
+        * solve_rel.
+        * eapply type_spine_const with (na :=nNamed "c") (A:=cat.(cat_obj)) (relevance:=r_obj).
+           ** eapply cumul_refl. simpl in *. eapply leq_refl.
+           ** solve_rel.
+           ** simpl. eapply type_spine_const with (na := nAnon) (A:=Hom(^1,^1)) (relevance:=r_hom).
+               *** eapply cumul_refl. simpl. eapply leq_refl.
+               *** apply id_hom_type. solve_rel.
+               *** simpl. eapply type_spine_const with
+                              (na := nAnon) (A:=Hom(^2,^1)) (relevance:=r_hom).
+                   **** eapply cumul_refl. simpl. eapply leq_refl.
+                   **** solve_rel.
+                   **** econstructor.
+Qed.
+
+Definition default_fctx (σ : list forcing_condition) : forcing_context := mkFCtxt σ cat [].
+
+Definition morphism_var_right' i n fctx : term :=
+  let q := get_domain_var fctx n in
+  morphism_var_alt_right cat q i (1+n) fctx.
+
+
+Notation "'φ(' q ',' i ',' n ',' σ ')'" :=
+  (morphism_var_alt_right cat q i (1+n) σ) (at level 20).
+
+(** This is a step of unfolding of the "morphism for the variable [n]" function.
+    See Def. 13 in the paper. This is a case for a morphism:
+    [ (σ ∙ (q,f))(x) = f ∘ σ(x) ]
+    Note, that in comparison with the paper, we use the usual order in the composition
+    ([g ∘ f] means "[g] after [f]")
+    Although, the proof is just refl, we keep it here to
+    show how variable indices are actually calculated when unfolding. *)
+Lemma morphism_var_unfold σ (σ' := [fcLift]) :
+  forall n q i,
+    φ(q,i,n,σ ∙ σ') = (^i) ∘ φ(q,2+i,n,σ) <:: [^q;^(2+i+σ.ₑ);^((σ ∙ σ').ₑ + i)].
+Proof.
+  intros n q i. reflexivity.
+Qed.
+
+Eval compute in (morphism_var_alt_right cat 0 1 0 [fcLift;fcVar;fcVar;fcLift;fcLift]).
+
+Lemma morphism_var_0 q σ cat : forall i,
+  morphism_var_alt_right cat q i 0 σ = tApp (cat_id cat) [^(i + get_domain_var_internal σ 0)].
+Proof.
+  induction σ;intros i.
+  - cbn. rewrite plus_0_r. reflexivity.
+  - simpl. destruct a.
+    * simpl. rewrite IHσ.
+      replace (S i + get_domain_var_internal σ 0)%nat with
+          (i + S (get_domain_var_internal σ 0))%nat by omega. reflexivity.
+    * simpl. replace (i+1)%nat with (S i) by omega. reflexivity.
+Qed.
+
+Lemma nat_compare_lt_Lt m n :
+  m < n ->
+  m ?= n = Lt.
+Proof.
+  intros;apply nat_compare_lt;omega.
+Qed.
+
+Lemma nat_compare_gt_Gt m n :
+  m > n ->
+  m ?= n = Gt.
+Proof.
+  intros;apply nat_compare_gt;omega.
+Qed.
+
+Lemma subst_morphism_gt t i j n σ q :
+  j <= 1 ->
+  j <= i ->
+  j <= q ->
+  φ(S q,S i,n,σ){j:=t} = φ(q,i,n,σ).
+Proof.
+  revert j. revert i. revert n.
+  induction σ.
+  - intros n i j Hj1 Hji Hjq.
+     simpl. rewrite nat_compare_lt_Lt by omega. reflexivity.
+  - intros n i j Hi1 Hji Hjq. destruct a.
+    + simpl. destruct n.
+      * repeat rewrite morphism_var_0. simpl.
+        rewrite nat_compare_lt_Lt by omega.
+        reflexivity.
+      * apply IHσ;auto.
+    + simpl. repeat rewrite nat_compare_lt_Lt by omega.
+      repeat f_equal. apply IHσ;auto.
+Qed.
+
+Lemma get_domain_var_sound uG (Σ := ([],uG)) Γ Γ' σ n :
+  (of_global_context Σ) ## Γ => Γ' |= σ ->
+  Σ ;;; Γ' |-  (^dom(σ,n)) : cat.(cat_obj).
+Proof.
+Admitted.
+
+Open Scope nat_scope.
+
+Lemma domain_var_last_condition_0 σ : get_domain_var_internal σ 0 = σ.ₑ.
+Proof.
+  induction σ.
+  - reflexivity.
+  - destruct a.
+    + simpl. congruence.
+    + reflexivity.
+Qed.
+
+Lemma domain_var_gt_0 σ n :
+  σ <> [] -> exists m, get_domain_var σ n = 1 + m.
+Proof.
+  Admitted.
+
+Lemma lift_morphism_var x σ q i :
+  lift0 1 (φ(q,i,x,σ)) = φ( 1 + q, 1+i, x, σ).
+Proof.
+  revert x. revert i.
+  induction σ; intros i x.
+  - reflexivity.
+  - destruct a.
+    + simpl.
+      destruct x.
+      * repeat rewrite morphism_var_0. reflexivity.
+      * rewrite IHσ. reflexivity.
+    + simpl. repeat f_equal. apply IHσ.
+Qed.
+
+Lemma morphism_var_sound_0 uG (Σ := ([],uG)) Γ Γ' σ x :
+  wf_graph uG ->
+  (of_global_context Σ) ## Γ => Γ' |= σ ->
+  Σ ;;; Γ' |- φ(dom(σ,x),0,x,σ) : Hom(^dom(σ,x), ^σ.ₑ).
+Proof.
+  intros Hwf FcValid.
+  revert x.
+  induction FcValid;intros x.
+  - cbn. apply id_hom_type. solve_rel.
+  - cbn. destruct x.
+    + rewrite morphism_var_0. rewrite domain_var_last_condition_0.
+      apply id_hom_type.
+      change (Σ;;; Γ' ,,, [v'] |- lift0 1 (^σ.ₑ) : lift0 1 (cat_obj cat)).
+      eapply weakening;auto. eapply last_condition_sound;eauto.
+    + change (Σ ;;; Γ' ,,, [v'] |- φ(1+dom(σ,x),1,x,σ) : lift0 1 Hom(^dom(σ,x), ^σ.ₑ)).
+      rewrite <- lift_morphism_var.
+      apply weakening. apply Hwf. apply IHFcValid.
+  - simpl. econstructor.
+    + eapply (cat_comp_type rlv_obj rlv_hom (nNamed "a") (nNamed "b") (nNamed "c")).
+    + eapply type_spine_const with (na :=nNamed "a") (A:=cat.(cat_obj)) (relevance:=rlv_obj).
+      * eapply cumul_refl. simpl in *. eapply leq_refl.
+      * eapply get_domain_var_sound;eauto. econstructor;eauto.
+      * eapply type_spine_const with (na :=nNamed "b") (A:=cat.(cat_obj)) (relevance:=rlv_obj).
+        ** eapply cumul_refl. simpl in *. eapply leq_refl.
+        ** pose [vass hom_name Relevant (tApp (tConst "Hom" []) [^S σ.ₑ; ^0]);
+                 vass pos_name Relevant (tConst "Obj" [])] as Γ''.
+           change (Σ;;; Γ' ,,, Γ''  |- lift0 2 (^(σ.ₑ)) : lift0 2 (cat_obj cat)).
+           apply weakening;auto. eapply last_condition_sound;eauto.
+        ** eapply type_spine_const with (na :=nNamed "c") (A:=cat.(cat_obj)) (relevance:=rlv_obj).
+           *** eapply cumul_refl. simpl in *. eapply leq_refl.
+           *** solve_rel.
+           *** simpl. eapply type_spine_const with (A:=Hom(^(2+σ.ₑ),^1))
+                                                   (relevance:=rlv_hom)(na:=nAnon).
+               **** eapply cumul_refl. simpl in *. rewrite Nat.eqb_refl.
+                    simpl. eapply leq_refl.
+               **** solve_rel.
+               **** simpl.
+                    eapply type_spine_const with (A:=Hom(^dom( σ ∙ [fcLift], x),^S (S σ.ₑ)))
+                                                 (relevance:=rlv_obj) (na:=nAnon).
+                    ***** eapply cumul_refl. simpl in *. rewrite Nat.eqb_refl. rewrite Nat.eqb_refl.
+                          simpl. eapply leq_refl.
+                    ***** simpl. unfold get_domain_var. simpl. repeat rewrite <- lift_morphism_var.
+                          setctx_2 Γ''.
+                          change (Σ;;; Γ' ,,, Γ'' |- ((lift0 1) ((lift0 1) (φ(dom(σ,x),0,x,σ)))) :
+                                                       lift0 2 (Hom(^dom(σ,x),^σ.ₑ))).
+                          rewrite <- simpl_lift.
+                          apply weakening;auto.
+                    ***** constructor.
+Qed.
+
+Fixpoint vars_fctx (n : nat) : list forcing_condition :=
+  match n with
+  | O => []
+  | S m => fcVar :: vars_fctx m
+  end.
+
+Definition nvars (σ : list forcing_condition) : nat :=
+  fold_right (fun fc i => match fc with fcVar => 1 + i | fcLift => i end) 0 σ.
+
+
+(** A generalization of morphism_var_sound_0 that works for any initial accumulator value [i] *)
+Lemma morphism_var_sound_i uG (Σ := ([],uG)) Γ Γ0 Γ' Γ'' σ x i :
+  wf_graph uG ->
+  (of_global_context Σ) ## Γ ,,, Γ0 => Γ' ,,, Γ'' |= (σ ∙ vars_fctx i) ->
+  #|Γ0| = i ->
+  #|Γ''| = i ->
+  Σ ;;; Γ' ,,, Γ'' |- φ(i+dom(σ,x),i,x,σ) : Hom(^(i+dom(σ,x)), ^(i+σ.ₑ)).
+Proof.
+  intros Hwf FcValid HΓ0 HΓ''.
+  generalize dependent Γ''. generalize dependent Γ0.
+  induction i;intros Γ0 HΓ0 Γ'' FcValid HΓ''.
+  - eapply morphism_var_sound_0;eauto.
+  - replace (S i + dom( σ, x)) with (1+(i + dom(σ,x))) by reflexivity.
+    rewrite <- lift_morphism_var.
+    destruct Γ''. inversion HΓ''. simpl in HΓ''.
+    destruct Γ0. inversion HΓ0. simpl in HΓ0.
+    change
+    (Σ;;; Γ',,,Γ'',,, [c] |-(lift0 1)(φ(i + dom(σ,x), i, x, σ)) : (lift0 1 (Hom(^((i + dom(σ,x))), ^(i + σ.ₑ))))).
+    apply weakening;auto.
+    eapply IHi. inversion HΓ0. reflexivity.
+    inversion FcValid;subst. eapply H0.
+    inversion HΓ''. reflexivity.
+Qed.
+
+
+Lemma last_cond_gt_0 σ v ψ : exists m, (σ ∙ [v] ∙ ψ).ₑ = 1+m.
+Proof.
+Admitted.
+
+Lemma last_condition_sum σ ψ :
+  only_vars ψ = true ->
+  (σ ∙ ψ).ₑ = fctx_size ψ + σ.ₑ.
+Proof.
+  intros H.
+  induction ψ.
+  - reflexivity.
+  - destruct a.
+    + simpl. rewrite IHψ;auto.
+    + inversion H.
+Qed.
+
+Lemma size_sum σ ψ :
+  fctx_size (σ ∙ ψ) = fctx_size σ + fctx_size ψ.
+Proof.
+  Admitted.
+
+Lemma last_condition_contains_lift σ ψ :
+  only_vars ψ = false ->
+  (σ ∙ ψ).ₑ = ψ.ₑ.
+Proof.
+  intros H.
+  induction ψ.
+  - inversion H.
+  - simpl. destruct a.
+    + simpl in *. rewrite IHψ;auto.
+    + reflexivity.
+Qed.
+
+Lemma size_gt_last_cond_lift σ :
+  only_vars σ = false ->
+  fctx_size σ > σ.ₑ.
+Proof.
+  intros H.
+  induction σ.
+  - inversion H.
+  - destruct a.
+    + simpl in H. simpl. assert (HH := IHσ H). omega.
+    + simpl. omega.
+Qed.
+
+Fixpoint condition_in (n : nat) (σ : list forcing_condition) : bool :=
+  match σ with
+  | [] => false
+  | fcVar :: σ' => condition_in (pred n) σ'
+  | fcLift :: σ' => if (Nat.eqb n 0) then true else condition_in n σ'
+  end.
+
+Lemma condition_in_contains_lift σ n :
+  condition_in n σ = true -> only_vars σ = false.
+Proof.
+  intros H.
+  generalize dependent n.
+  induction σ; intros n H.
+  - inversion H.
+  - destruct a.
+    + simpl in *. eauto.
+    + reflexivity.
+Qed.
+
+Lemma dom_condition_in_fctx σ ψ n :
+  condition_in (1+n) ψ = true -> dom(σ ∙ ψ,n) = dom(ψ,n).
+Proof.
+  intros H.
+  generalize dependent n.
+  induction ψ; intros n H.
+  - inversion H.
+  - destruct a.
+    + destruct n.
+      * cbn. do 2 rewrite domain_var_last_condition_0.
+        simpl in H.
+        assert (H1 : only_vars ψ = false) by (eapply condition_in_contains_lift;eauto).
+        change (S (σ ∙ ψ).ₑ = S ψ.ₑ).
+        rewrite last_condition_contains_lift;auto.
+      * cbn. apply f_equal. apply IHψ;auto.
+    + cbn. do 2 apply f_equal. simpl in H. apply IHψ;auto.
+Qed.
+
+Lemma fctx_size_gt_dom σ n :
+  condition_in (1+n) σ = true -> fctx_size σ > dom(σ,n).
+Proof.
+  revert n.
+  induction σ;intros n H.
+  - inversion H.
+  - destruct a.
+    + destruct n.
+      * simpl in H. simpl. unfold get_domain_var. simpl. apply gt_n_S.
+Admitted.
+
+Lemma fctx_size_lt_dom σ ψ n :
+  only_vars ψ = true ->
+  fctx_size ψ < dom(σ∙[fcLift]∙ψ,n).
+Proof.
+  revert n.
+  induction ψ;intros n Hv.
+  - cbn. omega.
+  - destruct a.
+    + unfold get_domain_var. simpl.
+      destruct n.
+      * rewrite domain_var_last_condition_0. simpl in Hv.
+        rewrite last_condition_sum by assumption. simpl. omega.
+      * simpl. apply gt_n_S. now apply IHψ.
+    + unfold get_domain_var. simpl. repeat apply gt_n_S. now apply IHψ.
+Qed.
+
+Lemma condition_in_0_contains_lift σ :
+  only_vars σ = false ->
+  condition_in 0 σ = true.
+Proof.
+  induction σ; intros H.
+  - inversion H.
+  - destruct a;easy.
+Qed.
+
+Lemma condition_in_0_only_vars σ :
+  condition_in 0 σ = false ->
+  only_vars σ = true.
+Proof.
+    induction σ; intros H.
+  - reflexivity.
+  - destruct a;easy.
+Qed.
+
+Lemma dom_0_eq_size σ :
+  only_vars σ = true ->
+  get_domain_var_internal σ 0 = fctx_size σ.
+Proof.
+  induction σ;intros.
+  - reflexivity.
+  - destruct a.
+    + simpl;easy.
+    + inversion H.
+Qed.
+
+Lemma dom_eq_size σ n :
+  condition_in (1+n) σ = false ->
+  dom(σ,n) = fctx_size σ.
+Proof.
+  revert n.
+  induction σ; intros n H.
+  - reflexivity.
+  - destruct a.
+    + unfold get_domain_var. simpl in *. apply f_equal.
+      destruct n.
+      * assert (only_vars σ = true) by now apply condition_in_0_only_vars.
+        now apply dom_0_eq_size.
+      * now apply IHσ.
+    + unfold get_domain_var. simpl in *. repeat apply f_equal.
+      now apply IHσ.
+Qed.
+
+(* WARNING: might be false in the peresent form and requires additional assumptions :) *)
+Lemma dom_lift_concat_only_vars_eq σ ψ n :
+  condition_in (1 + n) ψ = false ->
+  dom(σ∙[fcLift]∙ψ,n) = dom(σ∙ψ∙[fcLift],n).
+Proof.
+  revert n.
+  induction ψ; intros n H.
+  - reflexivity.
+  - destruct a.
+    + simpl in  H. cbn. apply f_equal.
+      destruct n.
+Admitted.
+
+Import Ring.
+
+Lemma dom_sum' σ ψ n :
+  only_vars ψ = true ->
+  get_domain_var_internal (σ∙ψ) n = fctx_size ψ + get_domain_var_internal σ (n-#|ψ|).
+Proof.
+  revert n.
+  induction ψ; intros n Hv.
+  - simpl in *. replace (n-0) with n by omega. reflexivity.
+  - destruct a.
+    + simpl in *. apply f_equal.
+      replace (n - S #|ψ|) with (pred n - #|ψ|) by omega.
+      now apply IHψ.
+    + simpl. inversion Hv.
+Qed.
+
+Lemma condition_in_0_n n σ:
+  condition_in 0 σ = false ->
+  condition_in n σ = false.
+Proof.
+  revert n.
+  induction σ; intros n H.
+  - reflexivity.
+  - destruct a.
+    + simpl in *. now apply IHσ.
+    + inversion H.
+Qed.
+
+Lemma dom_sum'' σ ψ n :
+  condition_in n ψ = false ->
+  exists m ,
+    get_domain_var_internal (σ∙ψ) n = fctx_size ψ + get_domain_var_internal σ m.
+Proof.
+  revert n.
+  induction ψ; intros n Hv.
+  - simpl in *. now eexists.
+  - destruct a.
+    + simpl in *. assert (HH:= IHψ _ Hv ).
+      destruct HH as [m Hm]. exists m. congruence.
+    + simpl in *. destruct n.
+      * inversion Hv.
+      * simpl in *.
+        simpl in *. assert (HH:= IHψ _ Hv ).
+        destruct HH as [m Hm].
+        exists m. congruence.
+Qed.
+
+Lemma dom_sum''' σ ψ n :
+  condition_in n ψ = false ->
+  1+nvars ψ > n ->
+  get_domain_var_internal (σ∙ψ) n = fctx_size ψ + get_domain_var_internal σ 0.
+Proof.
+  revert n.
+  induction ψ; intros n Hv Hvars.
+  - simpl in *. destruct n. reflexivity. inversion_clear Hvars. inversion H.
+  - destruct a.
+    + simpl.
+      (* apply gt_S_n in Hvars. *)
+      apply f_equal.
+      destruct n.
+      * simpl. repeat rewrite domain_var_last_condition_0.
+        rewrite last_condition_sum. omega.
+        now apply condition_in_0_only_vars.
+      * simpl. apply IHψ;auto. simpl in Hvars. omega.
+    + simpl in *. destruct n.
+      * inversion Hv.
+      * simpl in *.
+        simpl in *. repeat apply f_equal.
+        now apply IHψ.
+Qed.
+
+Lemma dom_sum_lift σ ψ n :
+  condition_in n ψ = false ->
+  1+nvars ψ > n ->
+  get_domain_var_internal (σ∙[fcLift]∙ψ) n = 1+fctx_size ψ.
+Proof.
+  intros. rewrite dom_sum''' by assumption. simpl.  omega.
+Qed.
+
+Lemma dom_sum σ ψ n :
+  only_vars ψ = true ->
+  dom(σ∙ψ,n) = fctx_size ψ + get_domain_var_internal σ (S n-#|ψ|).
+Proof.
+  intros.  now apply dom_sum'.
+Qed.
+
+Lemma fctx_size_gt_dom_lifts σ ψ n :
+  condition_in (1+n) ψ = false ->
+  fctx_size ψ < dom(σ∙[fcLift]∙ψ,n).
+Proof.
+  intros.
+  generalize dependent n.
+  induction ψ; intros n H.
+  - cbn. omega.
+  - destruct a.
+    + unfold get_domain_var. simpl in *.
+      destruct n.
+      * assert (only_vars ψ = true) by now apply condition_in_0_only_vars.
+        apply lt_n_S. rewrite domain_var_last_condition_0.
+        rewrite last_condition_sum by assumption.
+        simpl. omega.
+      * apply gt_n_S. now apply IHψ.
+    + unfold get_domain_var. simpl in *. repeat apply gt_n_S. now apply IHψ.
+Qed.
+
+
+Lemma fctx_size_gt_dom_lifts_S σ ψ n :
+  condition_in (1+n) ψ = false ->
+  nvars ψ <= n ->
+  1+fctx_size ψ < dom(σ∙[fcLift]∙ψ,n).
+Proof.
+  intros.
+  generalize dependent n.
+  induction ψ; intros n H Hvars.
+  - cbn. omega.
+  - destruct a.
+    + unfold get_domain_var. simpl in *.
+      destruct n.
+      * assert (only_vars ψ = true) by now apply condition_in_0_only_vars.
+        apply lt_n_S. rewrite domain_var_last_condition_0.
+        rewrite last_condition_sum by assumption.
+        simpl in *. inversion Hvars.
+      * apply gt_n_S. now apply IHψ.
+    + unfold get_domain_var. simpl in *. repeat apply gt_n_S. now apply IHψ.
+Qed.
+
+
+Conjecture congr_cumul_app_l : forall Σ Γ M1 M2 Ns,
+    cumul Σ Γ M1 M2 ->
+    cumul Σ Γ (tApp M1 Ns) (tApp M2 Ns).
+
+Conjecture congr_cumul_app_r : forall Σ Γ M Ns1 Ns2,
+    Forall2 (cumul Σ Γ) Ns1 Ns2 ->
+    cumul Σ Γ (tApp M Ns1) (tApp M Ns2).
+
+Tactic Notation "fold_ft_notation" :=
+  repeat
+    (match goal with
+     | |- context [(snd (otranslate (Environ.of_global_context ?Σ) (mkFCtxt ?σ ?cat []) ?v ?c))] =>
+       change (snd (otranslate (Environ.of_global_context Σ) (mkFCtxt σ cat []) v c))
+         with ([c]ᵗ Σ σ)
+     end).
+
+Tactic Notation "fold_morph_var_notation" :=
+  repeat
+    (match goal with
+     | |- context [morphism_var_alt_right ?cat ?q ?i (S ?n) ?σ] =>
+       change(morphism_var_alt_right cat q i (S n) σ) with (φ(q,i,n,σ))
+     end).
+
+Tactic Notation "fold_domain_var_notation" :=
+  repeat
+    (match goal with
+     | |- context [get_domain_var_internal ?fctx (S ?n)] => change (get_domain_var_internal fctx (S n)) with dom(fctx,n)
+     end).
+
+Tactic Notation "fold_fctx_notation" :=
+  repeat
+    (match goal with
+     | |- context [?xs ++ ?ys] =>
+       match type of xs with
+       | list forcing_condition => change (xs ++ ys) with (ys∙xs)
+       end
+     end).
+
+Tactic Notation "fold_fctx_notation_singleton" :=
+  repeat
+    (match goal with
+     | |- context [?x :: ?xs] =>
+       match type of x with
+       | forcing_condition =>
+         match xs with
+         | [] => idtac
+         | _ => change (x :: xs) with (xs∙[x])
+         end
+       end
+     | |- context [?x :: ?xs ∙ ?ys] =>
+       match type of x with
+       | forcing_condition =>
+         match xs with
+         | [] => idtac
+         | _ => change (x :: xs ∙ ys) with (xs∙[x]∙ys)
+         end
+       end
+     end).
+
+Tactic Notation "fold_fctx_notation_singleton1" :=
+  repeat
+    (match goal with
+     | |- context [?x :: ?xs ∙ ?ys] =>
+       match type of x with
+       | forcing_condition =>
+         match xs with
+         | [] => idtac
+         | _ => change (x :: xs ∙ ys) with (xs∙[x]∙ys)
+         end
+       end
+     end).
+
+Tactic Notation "fold_notation" :=
+  fold_morph_var_notation; fold_domain_var_notation;
+  fold_fctx_notation;fold_fctx_notation_singleton;fold_fctx_notation_singleton1;
+  fold_ft_notation.
+
+
+Tactic Notation "solve_cumul_refl" :=
+  eapply cumul_refl; simpl; repeat rewrite Nat.eqb_refl; (reflexivity || eapply leq_refl).
+
+
+(* Tries to solve as much as possible of the application:
+   [Σ ;;; Γ |- tApp M [N11;N12;N13...,N1n] <= tApp M [N21;N22;N23...,N2n]
+by applying congruence and resolving subgoals like [N1i <= N2i] by [cumul_refl] *)
+Ltac simpl_cumul_app_congr :=
+  let rec solve_rec := apply Forall2_cons;
+                       [> try solve_cumul_refl | (solve_rec ||apply Forall2_refl)]
+  in apply congr_cumul_app_r; solve_rec.
+
+Lemma morph_var_subst σ n uG (Σ := ([],uG)) Γ Γ' ψ :
+  let q := 1 + fctx_size ψ in
+  let f := fctx_size ψ in
+  cat_id_conv_l ->
+  wf_graph uG ->
+  (of_global_context Σ) ## Γ => Γ' |= (σ ∙ ψ) ->
+  Σ ;;; Γ' |- φ(dom(σ∙ψ,n),0,n, σ∙ψ) <= φ(dom(σ∙[fcLift] ∙ ψ,n),0,n,σ∙[fcLift]∙ψ){q:=^σ.ₑ}{f:= # ^σ.ₑ}.
+Proof.
+  intros ? ? id_left Hwf FcValid.
+  subst q. subst f.
+  revert n. generalize dependent Γ'. generalize dependent Γ.
+  induction ψ;intros Γ Γ' FcValid n.
+  - unfold get_domain_var. simpl.
+    erewrite subst_morphism_gt;eauto;try omega.
+    erewrite subst_morphism_gt;eauto;try omega.
+    eapply id_left.
+    econstructor.
+    + eapply (cat_comp_type rlv_obj rlv_hom (nNamed "a") (nNamed "b") (nNamed "c")).
+    + eapply type_spine_const with (na :=nNamed "a") (A:=cat.(cat_obj)) (relevance:=rlv_obj).
+      * eapply cumul_refl. simpl in *. eapply leq_refl.
+      * eapply get_domain_var_sound;eauto.
+      * eapply type_spine_const with (na :=nNamed "b") (A:=cat.(cat_obj)) (relevance:=rlv_obj).
+        ** eapply cumul_refl. simpl in *. eapply leq_refl.
+        ** eapply last_condition_sound;eauto.
+        ** eapply type_spine_const with (na :=nNamed "c") (A:=cat.(cat_obj)) (relevance:=rlv_obj).
+           *** eapply cumul_refl. simpl in *. eapply leq_refl.
+           *** eapply last_condition_sound;eauto.
+           *** simpl. eapply type_spine_const with (A:=Hom(^σ.ₑ,^σ.ₑ)) (na:=nAnon) (relevance:=rlv_hom).
+               **** eapply cumul_refl. simpl in *. rewrite Nat.eqb_refl.
+                    simpl. eapply leq_refl.
+               **** eapply id_hom_type. eapply last_condition_sound;eauto.
+               **** simpl.
+                    eapply type_spine_const with (A:=Hom(^get_domain_var_internal σ (S n),^σ.ₑ))
+                                                 (na:=nAnon)
+                                                 (relevance:=rlv_hom).
+                    ***** eapply cumul_refl. simpl in *. rewrite Nat.eqb_refl. rewrite Nat.eqb_refl.
+                          simpl. eapply leq_refl.
+                    ***** eapply morphism_var_sound_0;eauto.
+                    ***** constructor.
+  - destruct a.
+    + destruct n.
+      * simpl. repeat rewrite morphism_var_0.
+        repeat rewrite domain_var_last_condition_0. simpl.
+        destruct (last_cond_gt_0 σ fcLift ψ) as [m HH].
+        change (fcLift :: σ ∙ ψ) with (σ ∙ [fcLift] ∙ ψ).
+        rewrite HH.
+        destruct (only_vars ψ) eqn:Hψ.
+        ** simpl.
+           rewrite last_condition_sum in *;auto. simpl in HH.
+           assert (Hm : m = fctx_size ψ) by omega. subst m.
+           rewrite Nat.compare_refl. simpl.
+           rewrite nat_compare_lt_Lt by omega.
+           eapply cumul_refl. simpl in *. rewrite Nat.eqb_refl. reflexivity.
+        ** simpl. assert (Hσ' := last_condition_contains_lift (σ ∙ [fcLift]) _ Hψ).
+           assert (fctx_size ψ > ψ.ₑ) by (apply size_gt_last_cond_lift;auto).
+           rewrite nat_compare_gt_Gt by omega. simpl.
+           rewrite nat_compare_gt_Gt by omega.
+           eapply cumul_refl.
+           rewrite (last_condition_contains_lift σ) by assumption.
+           rewrite (last_condition_contains_lift (σ ∙ [fcLift])) in HH by assumption.
+           simpl. rewrite HH. rewrite Nat.eqb_refl. reflexivity.
+      * cbn. fold_notation.
+        repeat rewrite <- lift_morphism_var.
+        repeat rewrite commut_lift_subst.
+        inversion FcValid. subst.
+        change (Γ'0,, v') with (Γ'0 ,,, [v']).
+        apply weakening_cumul;auto.
+        eapply IHψ;eauto.
+    +  simpl. fold_notation.
+       assert (not_empty : (σ ∙ [fcLift] ∙ ψ) <> []).
+       { destruct ψ; unfold not; intros H; inversion H. }
+       destruct (domain_var_gt_0 (σ ∙ [fcLift] ∙ ψ) n not_empty) as [m HH].
+       rewrite HH.
+       destruct (last_cond_gt_0 σ fcLift ψ) as [m' HH'].
+       destruct (condition_in (1+n) ψ) eqn: Hψ.
+       simpl.
+       * rewrite dom_condition_in_fctx in HH by assumption.
+         assert (fctx_size ψ > dom(ψ,n)) by (apply fctx_size_gt_dom;auto).
+         rewrite nat_compare_gt_Gt by omega. simpl.
+         fold_notation.
+         rewrite dom_condition_in_fctx with (ψ :=ψ) by assumption.
+         rewrite nat_compare_gt_Gt by omega. simpl.
+         assert (Hψ' : only_vars ψ = false) by (eapply condition_in_contains_lift;eassumption).
+         fold_notation.
+         rewrite HH'. simpl.
+         assert (Hσ' := last_condition_contains_lift (σ ∙ [fcLift]) _ Hψ').
+         assert (fctx_size ψ > ψ.ₑ) by (apply size_gt_last_cond_lift;auto).
+         rewrite nat_compare_gt_Gt by omega. simpl.
+         rewrite nat_compare_gt_Gt by omega.
+         cbn. fold_notation.
+         replace (^S (S dom( σ ∙ ψ, n))) with (^S (S dom(ψ, n)))
+           by (now rewrite dom_condition_in_fctx).
+         replace (^S (S dom( (σ ∙ [fcLift]) ∙ ψ, n))) with (^S (S dom(ψ, n)))
+           by (now rewrite dom_condition_in_fctx).
+         rewrite (last_condition_contains_lift σ) by assumption.
+         rewrite (last_condition_contains_lift (σ ∙ [fcLift])) in HH' by assumption.
+         simpl in HH'. rewrite <- HH'.
+         simpl_cumul_app_congr.
+         inversion FcValid;subst.
+         repeat rewrite <- lift_morphism_var.
+         repeat rewrite commut_lift_subst. repeat rewrite <- simpl_lift.
+         apply weakening_cumul;auto.
+         now eapply IHψ.
+       * destruct (only_vars ψ) eqn:Hvψ.
+         ** destruct (le_lt_dec (nvars ψ) n) as [Hle | Hlt].
+            *** simpl.
+                assert (S (fctx_size ψ) < dom(σ∙[fcLift]∙ψ,n)) by now apply fctx_size_gt_dom_lifts_S.
+                rewrite nat_compare_lt_Lt by omega. simpl.
+                rewrite nat_compare_lt_Lt by omega.
+                replace (S m) with (dom(σ∙[fcLift]∙ψ,n)) by omega.
+                rewrite dom_lift_concat_only_vars_eq by assumption. simpl.
+                fold_notation.
+                rewrite HH'. simpl.
+                rewrite last_condition_sum in * by assumption. simpl in HH'.
+                assert (Hm : m' = fctx_size ψ) by omega. subst m'.
+                rewrite Nat.compare_refl. simpl.
+                rewrite nat_compare_lt_Lt by omega.
+                simpl_cumul_app_congr.
+                cbn. fold_notation.
+                inversion FcValid. subst.
+                repeat rewrite <- lift_morphism_var.
+                repeat rewrite commut_lift_subst.
+                repeat rewrite <- simpl_lift.
+                apply weakening_cumul;auto.
+                eapply IHψ;eauto.
+            *** simpl.
+                assert (Heq : fctx_size ψ = m).
+                { unfold get_domain_var in HH.
+                  rewrite dom_sum_lift in HH by assumption ||  omega. auto. }
+                rewrite Heq.
+                rewrite Nat.compare_refl. simpl.
+                rewrite nat_compare_lt_Lt by omega. rewrite <- Heq in *.
+                cbn. fold_notation.
+                assert (HltS : 1+nvars ψ > 1 +n) by omega.
+                assert (Hsum := dom_sum''' σ ψ _ Hψ HltS).
+                rewrite Hsum at 1.
+                simpl. rewrite domain_var_last_condition_0.
+                change (fcLift :: σ ∙ ψ) with (σ ∙ [fcLift] ∙ ψ).
+                rewrite HH'. simpl.
+                rewrite last_condition_sum in *;auto. simpl in HH'.
+                assert (Hm : m' = fctx_size ψ) by omega. subst m'.
+                rewrite Nat.compare_refl. simpl.
+                rewrite nat_compare_lt_Lt by omega.
+                simpl_cumul_app_congr.
+                fold_notation.
+                inversion FcValid. subst.
+                repeat rewrite <- lift_morphism_var.
+                repeat rewrite commut_lift_subst.
+                repeat rewrite <- simpl_lift.
+                apply weakening_cumul;auto.
+                eapply IHψ;eauto.
+         ** (* only_vars ψ = false *)
+            simpl.
+            destruct (le_lt_dec (nvars ψ) n) as [Hle | Hlt].
+            *** assert (S (fctx_size ψ) < dom(σ∙[fcLift]∙ψ,n)) by now apply fctx_size_gt_dom_lifts_S.
+                rewrite nat_compare_lt_Lt by omega.
+                simpl. rewrite nat_compare_lt_Lt by omega.
+                replace (S m) with (dom( (σ ∙ [fcLift]) ∙ ψ, n)) by omega.
+                rewrite dom_lift_concat_only_vars_eq by assumption.
+                cbn. fold_notation.
+                rewrite HH'. simpl.
+                assert (Hσ' := last_condition_contains_lift (σ ∙ [fcLift]) _ Hvψ).
+                assert (fctx_size ψ > ψ.ₑ) by (apply size_gt_last_cond_lift;auto).
+                rewrite nat_compare_gt_Gt by omega. simpl.
+                rewrite nat_compare_gt_Gt by omega.
+                rewrite (last_condition_contains_lift σ) by assumption.
+                rewrite (last_condition_contains_lift (σ ∙ [fcLift])) in HH' by assumption.
+                replace (S m') with ψ.ₑ by omega.
+                simpl_cumul_app_congr.
+                fold_notation.
+                inversion FcValid. subst.
+                repeat rewrite <- lift_morphism_var.
+                repeat rewrite commut_lift_subst.
+                repeat rewrite <- simpl_lift.
+                apply weakening_cumul;auto.
+                eapply IHψ;eauto.
+            *** assert (Heq : fctx_size ψ = m).
+                { unfold get_domain_var in HH.
+                  rewrite dom_sum_lift in HH by assumption ||  omega. auto. }
+                rewrite Heq. rewrite Nat.compare_refl. simpl.
+                rewrite nat_compare_lt_Lt by omega. rewrite <- Heq in *.
+                cbn. fold_notation.
+                assert (HltS : 1+nvars ψ > 1 +n) by omega.
+                assert (Hsum := dom_sum''' σ ψ _ Hψ HltS).
+                unfold get_domain_var at 1. rewrite Hsum.
+                simpl. rewrite domain_var_last_condition_0.
+                change (fcLift :: σ ∙ ψ) with (σ ∙ [fcLift] ∙ ψ).
+                rewrite HH'. simpl.
+                rewrite last_condition_contains_lift in *;auto. simpl in HH'.
+                assert (fctx_size ψ > ψ.ₑ) by now apply size_gt_last_cond_lift.
+                rewrite nat_compare_gt_Gt by omega. simpl.
+                rewrite nat_compare_gt_Gt by omega.
+                rewrite HH'. simpl.
+                simpl_cumul_app_congr.
+                fold_notation.
+                inversion FcValid. subst.
+                repeat rewrite <- lift_morphism_var.
+                repeat rewrite commut_lift_subst.
+                repeat rewrite <- simpl_lift.
+                apply weakening_cumul;auto.
+                eapply IHψ;eauto.
+Qed.
+
+(* TODO: Move to utils *)
+Lemma universe_equal_refl u :
+  Universe.equal u u = true.
+Proof.
+  induction u.
+  - reflexivity.
+  - simpl. rewrite univ_expr_eq_refl. auto.
+Qed.
+
+(* TODO: Move to utils *)
+Lemma eq_universe_refl g u :
+  eq_universe g u u = true.
+Proof.
+  unfold eq_universe.
+  rewrite universe_equal_refl. reflexivity.
+Qed.
+
+Lemma forcing_cond_subst_id uG (Σ := ([],uG)) t σ ψ Γ Γ' :
+  let q := 1 + fctx_size ψ in
+  let f := fctx_size ψ in
+  cat_id_conv_l ->
+  wf_graph uG ->
+  (of_global_context Σ) ## Γ => Γ' |= (σ ∙ ψ) ->
+  Σ ;;; Γ' |- ([t]ᵗ Σ (σ∙ψ)) <= ([t]ᵗ Σ (σ∙[fcLift]∙ψ)){q:=^σ.ₑ}{f:= # ^σ.ₑ}.
+Proof.
+  induction t;intros ? ? id_left Hwf FCvalid.
+  - (* tRel *)
+    unfold ft_term,otranslate,snd. unfold translate_var. unfold morphism_var_right.
+    replace (1+n) with (S n) by reflexivity. fold_notation. simpl.
+    admit.
+    (* NOTE: if we want to prove this for any [ψ], we first should show some
+       properties of [get_var_sift]*)
+    (* simpl_cumul_app_congr. fold_notation. *)
+    (* change (Σ;;; Γ' |- φ(dom(σ∙ψ,n),0,n,σ∙ψ) <=  φ(dom(σ∙[fcLift]∙ψ,n),0,n, σ∙[fcLift]∙ψ) {q := ^σ.ₑ} {f := # ^σ.ₑ}). now eapply morph_var_subst with (ψ := [fcLift]). *)
+  - admit. (* [tVar] not supported*)
+  - admit. (* [tMeta] not supported*)
+  - admit. (* [tEvar] not supported*)
+  - (* tSort *) constructor. simpl. admit.
+                (* apply eq_universe_refl. *)
+Admitted.
+
+Lemma forcing_typing_soundness uG (Σ := ([],uG)) Γ Γ' t T σ :
+  cat_id_conv_l ->
+  wf_graph uG ->
+  (of_global_context Σ) ## Γ => Γ' |= σ ->
   Σ ;;; Γ |- t : T ->
   let Σ' := Σ in
-  Σ' ;;; (⟦Γ⟧ Σ σ) |- ([t]ᵗ Σ σ) : (⟦T⟧ᵀ Σ σ).
+  Σ' ;;; Γ' |- ([t]ᵗ Σ σ) : (⟦T⟧ᵀ Σ σ).
 Proof.
-  intros TyCtx Ty.
-  revert σ.
-  induction Ty; intros; simpl.
+  intros id_left wfG FcValid Ty.
+  generalize dependent Γ'.
+  generalize dependent σ.
+  induction Ty; intros σ Γ' FcValid; simpl.
   - (* -- Variables -- *)
-    simpl. unfold translate_var.
-    unshelve econstructor; simpl.
-    Focus 2. constructor.  admit.
+    simpl. unfold ft_term,ft_type. simpl. unfold translate_var. simpl.
+    eapply type_Conv.
+    + eapply type_App.
+      * (* something about [get_var_shift] with relation to the valid forcing context *)  admit.
+      * (* stuff about [morph_var]  *) admit.
+    + admit.
+    + admit.
   - (* -- Sorts -- *)
-    assert (FcValid : of_global_context Σ ## (⟦ Γ ⟧) Σ σ |= σ) by
-        (apply context_traslation_valid;auto).
-    (* Simplifying the applications in the type first*)
-      unfold ft_term,otranslate,lambda_prefix,extend.
-      eapply type_Conv;simpl.
-      * apply lam_q_f_sound;simpl.
-        ** apply forcing_context_soundness;assumption.
-        ** apply FcValid.
-        ** eapply Π_q_f_lift_sound; apply type_Sort.
-      * unfold ft_type. simpl in *. unfold mkOptApp.
-        eapply type_App.
-        ** eapply lam_q_f_sound;simpl.
-           *** apply forcing_context_soundness;assumption.
-           *** apply FcValid.
-           *** apply Π_q_f_lift_sound. unfold Universe.super. simpl.
-               unfold Universe.type1,Universe.Expr.type1.
-           (* TODO: show that [tSort [(Level.set, true)]] has type [tSort l] for some level l *)
-           (* constructor [type_Sort] does not apply here. *)
-               admit.
-        ** simpl. (* typing_spine *)
-           type_spine_step. solve_last_cond.
-           type_spine_step. apply id_hom_type. solve_last_cond.
-           apply type_spine_nil.
-      * simpl. unfold ft_type. simpl. unfold mkOptApp.
-        (* Abstract this reduction to a tactic *)
-        eapply cumul_red_r. Focus 2.
-        eapply red_beta. simpl.
-        eapply cumul_red_r. Focus 2.
-        eapply red_beta. simpl.
-        eapply cumul_refl.
-        simpl.
-        (* NOTE: not sure how to prove this stuff about [leq_universe] *)
-        assert (H : leq_universe
-                      init_graph
-                      (Universe.sup [Universe.Expr.set]
-                                    (Universe.sup [Universe.Expr.set] (Universe.super l)))
-                      (Universe.super l) = true). admit.
-        rewrite H. rewrite Nat.eqb_refl. reflexivity.
+    eapply translation_of_sort_sound with
+        (s' := (Universe.super l));eauto.
+    (* Admit for now assumptions about how the universe levels are related. *)
+    admit.
+    admit.
   - admit.
   - (* -- Products -- *)
-    assert (CtxSound : type_local_env Σ (⟦Γ⟧ Σ σ)) by (apply forcing_context_soundness;auto).
-    assert (FcValid : of_global_context Σ ## (⟦ Γ ⟧) Σ σ |= σ) by
-        (apply context_traslation_valid;auto).
-    rename t into A. rename b into B.
-    unfold ft_type, ft_term,snd. simpl.
-    destruct (otranslate_boxed_type otranslate (of_global_context Σ)
-            (extend_forcing_ctx {| f_context := σ; f_category := cat; f_translator := nil |} fcLift)
-            tt A) as [sigma t_] eqn:Ht.
-    destruct (otranslate_type otranslate (of_global_context Σ)
-            (add_variable
-               (extend_forcing_ctx {| f_context := σ; f_category := cat; f_translator := nil |}
-                                   fcLift)) sigma B) as [sigma0 u_] eqn:Hu.
-    unfold mkOptApp.
-    eapply type_Conv;simpl.
-    * eapply lam_q_f_sound;simpl.
-      ** apply forcing_context_soundness;assumption.
-      ** apply FcValid.
-      ** eapply type_Prod.
-         *** eapply Π_q_f_lift_sound.
-             eapply type_translation_sound.
-             **** simpl.
-                  pose [vass hom_name Relevant (tApp cat_hom [tRel 2; tRel 0]);
-                        vass pos_name Relevant cat_obj] as Γ'.
-                  pose [vass hom_name Relevant (tApp cat_hom [tRel (S (last_condition σ)); tRel 0]);
-                        vass pos_name Relevant (tConst "Obj" [])] as Γ''.
-                  change (type_local_env ([], init_graph) (⟦ Γ ⟧ Σ σ ,,, Γ'' ,,, Γ')).
-                  eapply ctx_with_lift_sound with (σ := σ ,, fcLift);eauto.
-                  eapply ctx_with_lift_sound with (σ := σ);eauto.
-                  constructor;eauto.
-             **** repeat constructor;eauto.
-             **** simpl.
-                  pose [vass hom_name Relevant (tApp cat_hom [tRel 2; tRel 0]);
-                        vass pos_name Relevant cat_obj] as Γ'.
-                  pose [vass hom_name Relevant (tApp cat_hom [tRel (S (last_condition σ)); tRel 0]);
-                        vass pos_name Relevant (tConst "Obj" [])] as Γ''.
-                  assert (Hs1 :[Universe.Expr.set] = s1). admit.
-                  rewrite Hs1. simpl in IHTy1.
-                  change
-  (Σ ;;; (⟦ Γ ⟧) Σ σ ,,, Γ'' ,,, Γ' |- [A ]ᵗ Σ (σ,, fcLift,, fcLift) : (⟦ tSort s1 ⟧ᵀ Σ  (σ,, fcLift,, fcLift))).
-                  pose ((⟦ Γ ⟧) Σ ((σ,, fcLift),, fcLift)) as G.
-                  unfold ft_ctx in G.
-                  (* assert (Hfc : of_global_context Σ ## G |= (σ ,, fcLift ,, fcLift)). *)
-                  (* { constructor. } *)
-                  (* simpl in G. *)
-                  (* eapply IHTy1 with (σ := σ ,,fcLift,,fcLift). *)
-                  admit.
-
+    eapply prod_translation_sound.
+    * exact wfG.
+    * eapply FcValid.
+    * apply IHTy1;repeat constructor;auto.
+    * apply IHTy2;repeat constructor;auto.
+  - (* -- Lambda -- *)
+    pose (get_ctx_lift cat (of_global_context Σ) (last_condition σ)) as ext.
+    pose (σ ,, fcLift) as σ'.
+    assert
+    (TyCtxExt' : type_local_env Σ (Γ' ,,, ext ,, vass n relevance (⟦t⟧! Σ σ'))).
+    { constructor.
+      * (* NOTE: here we need the fact that [Γ'] is well-formed *) admit.
+      * fold (app (A:=context_decl)). econstructor.
+        unfold decl_type,vass.
+        eapply boxed_type_translation_sound.
+        ** exact wfG.
+        ** repeat constructor;eauto.
+        ** eapply IHTy1;eauto;repeat constructor;auto. }
+    assert
+      ( Tyb_tr : Σ;;; Γ' ,,, ext ,, vass n relevance (⟦t⟧! Σ σ') |-
+        [b]ᵗ Σ (σ' ,, fcVar) : (⟦ bty ⟧ᵀ) Σ (σ' ,, fcVar)).
+    { eapply IHTy2 with (Γ':=Γ' ,,, ext ,, vass n relevance (⟦t⟧! Σ σ')).
+      constructor;eauto. eapply fctx_valid_cons_lift. eauto. }
+    destruct (typed_term_sort uG _
+             ([b ]ᵗ Σ (σ' ,, fcVar)) (⟦ bty ⟧ᵀ Σ (σ' ,, fcVar)) TyCtxExt' wfG Tyb_tr) as [s Hs].
+    evar (s' : universe).
+    assert (Ty_bty : Σ;;; Γ' |- (⟦ tProd n relevance t bty ⟧ᵀ) Σ σ : tSort ?s').
+    { eapply type_translation_sound;eauto.
+      eapply prod_translation_sound_alt;eauto.
+      ** eapply boxed_type_translation_sound.
+         *** exact wfG.
+         *** repeat constructor;eauto.
+         *** eapply IHTy1;eauto;repeat constructor;auto. }
+    (* unfold ft_type, ft_term. simpl. *)
+    eapply type_Conv;eauto.
+    * eapply type_Lambda;fold otranslate in *.
+      ** eapply boxed_type_translation_sound.
+         *** exact wfG.
+         *** repeat constructor;eauto.
+         *** apply IHTy1;eauto.
+             repeat constructor;eauto.
+      ** setctx Γ''.
+         assert (H : Σ;;; Γ'' |- [b ]ᵗ Σ (σ ,, fcVar) : (⟦ bty ⟧ᵀ) Σ (σ ,, fcVar)).
+         { eapply IHTy2 with (σ := σ,,fcVar) (Γ':=Γ'').
+           change (of_global_context Σ ## Γ,, vass n relevance t =>
+                   Γ' ,, vass n relevance (⟦t⟧! Σ σ) |= σ,, fcVar).
+           eapply fctx_valid_cons_var;eauto. }
+         unfold ft_term in H.
+         erewrite <- unit_unique in H.
+         eapply H.
+    * (* NOTE: do something with names *)
+      assert (Eq_names : n = n'). admit.
+      rewrite Eq_names in Ty_bty. apply Ty_bty.
+    * fold otranslate. instantiate (1:=n').
+      change (Σ;;; Γ' |- tProd n' relevance (⟦t⟧! Σ σ)
+       ((⟦ bty ⟧ᵀ) Σ (σ,, fcVar)) <= (⟦ tProd n' relevance t bty ⟧ᵀ) Σ σ).
+      eapply cumul_red_r. Focus 2. unfold ft_type,mkOptApp,otranslate_type,snd. simpl.
+      eapply red_beta. simpl.
+      eapply cumul_red_r. Focus 2.
+      eapply red_beta. simpl.
+      apply congr_cumul_prod.
+      ** apply congr_cumul_prod. eapply cumul_refl;auto.
+         simpl. apply congr_cumul_prod.
+         *** eapply cumul_refl;auto. simpl. rewrite Nat.eqb_refl. reflexivity.
+         *** apply congr_cumul_app_l.
+             change (Σ ;;; Γ' ,,, ext |-  ([t ]ᵗ Σ σ') <=
+                                          (([t]ᵗ Σ (σ'∙[fcLift])){3 :=^σ.ₑ}{2 := # ^σ.ₑ})).
+             assert (FcValid' : of_global_context Σ ## Γ => Γ' ,,, ext |= (σ ∙ [fcLift])) by
+                  (repeat econstructor;eauto).
+             now apply forcing_cond_subst_id with (ψ:=[fcLift]) (Γ:=Γ).
+      ** unfold ft_type. simpl. unfold mkOptApp. simpl.
+         unfold add_variable,extend_forcing_ctx. simpl.
+         pose (vass n' relevance ((⟦ t ⟧!) Σ σ)) as v'.
+         pose (vass n relevance t) as t'.
+         assert (H : Σ;;; Γ',, v' |- tApp ([bty ]ᵗ Σ (σ∙[fcVar])) [^S σ.ₑ; # ^S σ.ₑ] <=
+                                 tApp (([bty ]ᵗ Σ (σ∙[fcLift]∙[fcVar])){2:=^σ.ₑ}{1:=# ^σ.ₑ})
+                                      [^S σ.ₑ; # (^S σ.ₑ)]).
+         eapply congr_cumul_app_l.
+         assert (FcValid' : of_global_context Σ ## Γ ,, t' => Γ' ,, v' |= (σ ∙ [fcVar]))
+           by (repeat econstructor;eauto).
+         now apply forcing_cond_subst_id with (Γ:=Γ,,t').
+         unfold ft_term in H. erewrite <- unit_unique in H at 2.
+         eapply H.
+  - (* tLetIn *)
+      admit.
 Admitted.
