forcing/Demo.v
@@ -1,0 +1,135 @@
+Require Import Template.monad_utils Template.Ast Template.AstUtils
+        Template.Template Template.LiftSubst.
+Require Import Forcing.TemplateForcing.
+Require Import Forcing.translation_utils.
+Require Import List.
+Require Import Template.Typing.
+
+
+(* To be able to work with values in SProp we define boxing/unboxing *)
+Inductive sBox (A : SProp) : Prop := sbox : A -> sBox A.
+
+Definition ubox {A : SProp} (bA : sBox A) : A :=
+  match bA with
+    sbox _ X => X
+  end.
+
+
+Inductive sle : nat -> nat -> SProp :=
+  sle_0 : forall n, sle 0 n
+| sle_S : forall n m : nat, sle n m -> sle (S n) (S m).
+
+Inductive sFalse : SProp :=.
+
+Inductive sTrue : SProp := I.
+
+Definition sle_refl (n : nat) : sle n n.
+Proof.
+  induction n;constructor;auto.
+Qed.
+
+Lemma sle_Sn_0 : forall n, sle (S n) 0 -> sFalse.
+Proof.
+  unfold Hom; intros n H.
+  inversion H.
+Qed.
+
+Definition sle_Sn (n : nat) : sle n (S n).
+Proof.
+  induction n; constructor; auto.
+Qed.
+
+
+Definition sle_trans {n m p} (H : sle n m) (H': sle m  p) : sle n p.
+Proof.
+  revert H'. revert p. induction H.
+  - intros p H'. apply sle_0.
+  - intros p H'. inversion H'.
+    apply ubox. subst. apply sbox.
+    apply sle_S. apply IHsle;auto.
+Qed.
+
+(* A category of forcing conditions *)
+(* NOTE: we define ℕop *)
+
+Definition nat_obj : Type := nat.
+Definition nat_hom (P Q : nat_obj): SProp := sle Q P.
+Notation "P ≥ Q" := (nat_hom P Q) (at level 70).
+
+Definition nat_id_hom (P : nat_obj) : P ≥ P := sle_refl P.
+Notation "# R" := (nat_id_hom R) (at level 70).
+
+Definition nat_comp (A B C : nat_obj) (g : B ≥ C) (f : A ≥ B) : A ≥ C
+  := sle_trans  g f.
+
+Notation "g ∘ f" := (nat_comp _ _ _ g f) (at level 40).
+
+Arguments sbox {_}.
+
+(* Now, laws hold definitionally, thanks to SProp *)
+(* We use sbox'ed version to prove this *)
+Lemma nat_cat_left_id P R (g : R ≥ P)  : sbox (g ∘ (# _)) = sbox g.
+Proof. reflexivity. Qed.
+
+Lemma nat_cat_right_id P R (f : P ≥ R)  : sbox (f ∘ (# _)) = sbox f.
+Proof. reflexivity. Qed.
+
+Lemma nat_cat_assoc P Q R S (f : S ≥ Q) (g : R ≥ S) (h : P ≥ R):
+  sbox (f ∘ (g ∘ h)) = sbox ((f ∘ g) ∘ h).
+Proof. reflexivity. Qed.
+
+Quote Definition q_nat_obj := nat_obj.
+Quote Definition q_nat_hom := nat_hom.
+Quote Definition q_id_nat_hom := nat_id_hom.
+Quote Definition q_nat_comp := nat_comp.
+
+
+(** A category of nat with the ordering *)
+Definition nat_cat : category :=
+  mkCat q_nat_obj q_nat_hom q_id_nat_hom q_nat_comp.
+
+(** An instance for the monad *)
+Instance GuardRec : Translation := ForcingTranslation nat_cat.
+
+Import ListNotations.
+Import MonadNotation.
+Open Scope string_scope.
+
+Set Printing Universes.
+
+Check SProp.
+
+Inductive s_and (A B : SProp) : SProp :=  conj : A -> B -> s_and A B.
+
+Check (forall p : SProp, s_and p p).
+
+Check (forall p : Type, prod p p).
+
+(* Initial context *)
+Run TemplateProgram (prg <- tmQuoteRec nat_hom ;;
+                     tmDefinition "g_ctx" (fst prg)).
+Definition ΣE : tsl_context:= (reconstruct_global_context g_ctx,[]).
+
+Definition tTranslateTy {tsl : Translation} (ΣE : tsl_context)
+           (id : ident) (A : Type)
+  : TemplateMonad (tsl_context) :=
+  tA <- tmQuote A ;;
+  tA' <- tmEval lazy (tsl_ty ΣE tA) ;;
+  match tA' with
+  | Error e => print_nf e ;; fail_nf ("Translation error during the translation of the type of " ++ id)
+  | Success tA' =>
+      id' <- tmEval all (tsl_id id) ;;
+      A' <- tmUnquoteTyped Type tA' ;;
+
+
+Run TemplateProgram (tTranslateTy ΣE "later_type" (Type->Type)).
+
+Run TemplateProgram (tImplementTC ΣE "later_TC" "later" (Type->Type)).
+Next Obligation.
+  destruct p0.
+  - exact unit.
+  - exact (X p0 (sle_Sn p0 ∘ H) p0 (# _)).
+Defined.
+
+Print later.
+Print laterᵗ_obligation_1.
